finishing proofs with the properties. using a global property set for now
Signed-off-by: Reto Achermann <reto.achermann@inf.ethz.ch>

theories/model/Syntax.thy
@@ -45,13 +45,13 @@ record block_spec =
   base    :: genaddr
   limit   :: genaddr
   require :: "property list"
-  forbid  :: "property list"
+  reject  :: "property list"
 
 definition block :: "genaddr \<Rightarrow> genaddr \<Rightarrow> property list \<Rightarrow> property list \<Rightarrow> block_spec"
-  where "block b l r f  = \<lparr> base = b, limit = l, require = r, forbid = f \<rparr>"
+  where "block b l r f  = \<lparr> base = b, limit = l, require = r, reject = f \<rparr>"
 
 definition blockn :: "genaddr \<Rightarrow> genaddr \<Rightarrow> block_spec"
-  where "blockn b l  = \<lparr> base = b, limit = l, require = [], forbid = [] \<rparr>"
+  where "blockn b l  = \<lparr> base = b, limit = l, require = [], reject = [] \<rparr>"
 
 
 
@@ -60,27 +60,38 @@ text {* For each syntax item (nonterminal), we have a translation function into
         of \autoref{sec:reductions}. *}
 
 
+
+text {* An address contains a set of properties. When specifying a set of addresses
+        that are translated or accepted we use the notion of required and rejected properties. 
+        An address that is element of the accept or translate set must fulfill the following
+        predicate. *}
+
 definition prop_pred :: "property set \<Rightarrow> property set \<Rightarrow> property set \<Rightarrow> bool"
   where "prop_pred incl excl props =  (excl \<inter> props = {}  \<and> incl \<subseteq> props)"
 
 
-definition mk_block :: "block_spec \<Rightarrow> addr set"
-  where "mk_block s = {(a, p) | a p. (base s) \<le> a \<and> a \<le> (limit s) 
-                                \<and> prop_pred (set (require s)) (set (forbid s)) p }"
-
-lemma "\<forall>P. \<exists>I. prop_pred A B P \<longleftrightarrow> prop_pred A B (P-I)"
-  by(auto simp:prop_pred_def)
-  
-
-definition  wf_mkblock :: "block_spec \<Rightarrow> bool" 
-  where  "wf_mkblock s = (\<exists>n. \<forall>ap \<in> mk_block s. (snd ap) < n)"
+text {* When creating the block from it's spec we include a set of net properties which are the
+        properties mentioned in the decoding net and therefore the properties we care about. *}
 
 
-  
+definition mk_block :: "property set \<Rightarrow> block_spec \<Rightarrow> addr set"
+  where "mk_block netpropss s = {(a, p) | a p. (base s) \<le> a \<and> a \<le> (limit s) 
+                                   \<and> prop_pred (set (require s)) (set (reject s)) p
+                                   \<and> p \<subseteq> netpropss }"
+
+
+text {* We obtain the relevant properties of a block by the union of the reject and require lists *}
+
+
+primrec mk_block_propset :: "block_spec list \<Rightarrow> property set"
+  where "mk_block_propset [] = {}" |
+        "mk_block_propset (m#mm) = (mk_block_propset mm) \<union> set (require m) \<union> set (reject m)"
+
 
 
 text {* A single block mapping that maps the specified source block to the given 
-        destination node, beginning at the given base address: *}
+        destination node, beginning at the given base address and adds or strips some 
+        properties. *}
 
 
 record map_spec =
@@ -118,7 +129,7 @@ definition direct_map_p :: "block_spec \<Rightarrow> nodeid \<Rightarrow> proper
 
 definition one_map :: "addr \<Rightarrow> nodeid \<Rightarrow> genaddr \<Rightarrow> map_spec"
   where "one_map src nd ba =  \<lparr> src_block = \<lparr> base = (fst src), limit = (fst src), 
-                                             require = [], forbid = [] \<rparr>,
+                                             require = [], reject = [] \<rparr>,
                                dest_node = nd, dest_base = ba,
                                propadd =[],propstrip = [] \<rparr>"
 
@@ -127,18 +138,28 @@ definition one_map_p :: "addr \<Rightarrow> nodeid \<Rightarrow> genaddr \<Right
   where "one_map_p src nd ba pa ps =  \<lparr> src_block = \<lparr> base = (fst src), 
                                                      limit = (fst src), 
                                                      require = [], 
-                                                     forbid = [] \<rparr>,
+                                                     reject = [] \<rparr>,
                                        dest_node = nd, dest_base = ba,
                                        propadd =  pa,propstrip =  ps \<rparr>"
 
 
-definition mk_map :: "map_spec \<Rightarrow> addr \<Rightarrow> name set"
-  where "mk_map s =
-    (\<lambda>a. if a \<in> mk_block (src_block s)
+definition mk_map :: "property set \<Rightarrow> map_spec \<Rightarrow> addr \<Rightarrow> name set"
+  where "mk_map ps s =
+    (\<lambda>a. if a \<in> mk_block ps (src_block s)
       then {
         (dest_node s, (dest_base s + (fst a - base (src_block s))), 
                          (snd a) \<union> (set (propadd s)) - (set (propstrip s))) }
       else {})"
+
+
+text {* we can obtain the relevant properties of the map by the union of the propadd, propetrip
+        and source block properties *}
+
+
+primrec mk_map_propset :: "map_spec list \<Rightarrow> property set"
+  where "mk_map_propset [] = {}" |
+        "mk_map_propset (m#mm) = (mk_map_propset mm) \<union> set (propadd m) 
+                                      \<union> set (propstrip m) \<union> mk_block_propset [src_block m]"
 
 
 
@@ -175,76 +196,76 @@ lemma accept_mk_overlay:
   by(simp add:mk_overlay_def)
 (*>*)
 
-primrec add_blocks :: "block_spec list \<Rightarrow> node \<Rightarrow> node"
-  where "add_blocks [] node = node" |
-        "add_blocks (s#ss) node = accept_update (op \<union> (mk_block s)) 
-                                                (add_blocks ss node)"
+primrec add_blocks :: "property set \<Rightarrow> block_spec list \<Rightarrow> node \<Rightarrow> node"
+  where "add_blocks ps [] node = node" |
+        "add_blocks ps (s#ss) node = accept_update (op \<union> (mk_block ps s)) 
+                                                   (add_blocks ps ss node)"
 
 
 
 (*<*)
 lemma translate_add_blocks:
-  "translate (add_blocks bs node) = translate node"
+  "translate (add_blocks ps bs node) = translate node"
   by(induct bs, simp_all)
 
 lemma add_blocks_overlay:
-  "accept (add_blocks bs (mk_overlay ov)) =
-   accept (add_blocks bs empty_node)"
+  "accept (add_blocks ps bs (mk_overlay ov)) =
+   accept (add_blocks ps bs empty_node)"
   by(induct bs, simp_all add:empty_node_def accept_mk_overlay)
 (*>*)
 
-definition add_maps :: "map_spec list \<Rightarrow> node \<Rightarrow> node"
-  where "add_maps ss node = translate_update 
-                                (\<lambda>t a. \<Union>{mk_map s a |s. s\<in>(set ss) } \<union> t a) 
-                                node"
+definition add_maps :: "property set \<Rightarrow> map_spec list \<Rightarrow> node \<Rightarrow> node"
+  where "add_maps ps ss node = translate_update 
+                                   (\<lambda>t a. \<Union>{mk_map ps s a |s. s\<in>(set ss) } \<union> t a) 
+                                    node"
     
-primrec add_maps_rec :: "map_spec list \<Rightarrow> node \<Rightarrow> node"
-  where "add_maps_rec [] node = node" |
-        "add_maps_rec (s#ss) node = translate_update 
-                                      (\<lambda>t a. mk_map s a \<union> t a) 
-                                      (add_maps_rec ss node)"    
+primrec add_maps_rec :: "property set \<Rightarrow> map_spec list \<Rightarrow> node \<Rightarrow> node"
+  where "add_maps_rec ps [] node = node" |
+        "add_maps_rec ps (s#ss) node = translate_update 
+                                          (\<lambda>t a. mk_map ps s a \<union> t a) 
+                                          (add_maps_rec ps ss node)"    
 
 
-definition remove_maps :: "map_spec list \<Rightarrow> node \<Rightarrow> node"
-  where "remove_maps ss node = translate_update 
-                                   (\<lambda>t a. t a - \<Union>{mk_map s a |s. s\<in>(set ss) }) 
+definition remove_maps :: "property set \<Rightarrow> map_spec list \<Rightarrow> node \<Rightarrow> node"
+  where "remove_maps ps ss node = translate_update 
+                                   (\<lambda>t a. t a - \<Union>{mk_map ps s a |s. s\<in>(set ss) }) 
                                     node"
 
 lemma remove_maps_set_diff: 
-  "A - \<Union>{mk_map s a |s. s \<in> set ms \<or> s \<in> set ns} 
-    = A - \<Union>{mk_map s a |s. s \<in> set ns} - \<Union>{mk_map s a |s. s \<in> set ms}"
+  "A - \<Union>{mk_map ps s a |s. s \<in> set ms \<or> s \<in> set ns} 
+    = A - \<Union>{mk_map ps s a |s. s \<in> set ns} - \<Union>{mk_map ps s a |s. s \<in> set ms}"
   by(auto)      
 
 
 lemma remove_maps_append :
-  "remove_maps (ms @ ns) node = remove_maps ms (remove_maps ns node)"
+  "remove_maps ps (ms @ ns) node = remove_maps ps ms (remove_maps ps ns node)"
   by(auto simp add:remove_maps_def o_def remove_maps_set_diff)    
     
         
-definition add_one_map :: "map_spec \<Rightarrow> node \<Rightarrow> node"
-  where "add_one_map m n = translate_update (\<lambda>t a. mk_map m a \<union> t a) n"
+definition add_one_map :: "property set \<Rightarrow> map_spec \<Rightarrow> node \<Rightarrow> node"
+  where "add_one_map ps m n = translate_update (\<lambda>t a. mk_map ps m a \<union> t a) n"
 
-definition remove_one_map :: "map_spec \<Rightarrow> node \<Rightarrow> node"
-  where "remove_one_map m n = n \<lparr> translate := (\<lambda>a. translate n a - mk_map m a) \<rparr>"
+definition remove_one_map :: "property set \<Rightarrow> map_spec \<Rightarrow> node \<Rightarrow> node"
+  where "remove_one_map ps m n = n \<lparr> translate := (\<lambda>a. translate n a - mk_map ps m a) \<rparr>"
     
-definition update_one_map :: "map_spec \<Rightarrow> map_spec \<Rightarrow> node \<Rightarrow> node"
-  where "update_one_map m m' n = add_one_map m' (remove_one_map m n)"        
+definition update_one_map :: "property set \<Rightarrow> map_spec \<Rightarrow> map_spec \<Rightarrow> node \<Rightarrow> node"
+  where "update_one_map ps m m' n = add_one_map ps m' (remove_one_map ps m n)"        
 
 
 lemma update_commute:
-  assumes m_distinct: "\<And>a. translate node a \<inter> mk_map m a = {}"
-      and n_contained: "\<And>a. mk_map n a \<subseteq> translate node a"
-  shows "update_one_map m n (update_one_map n m node) = node"
+  assumes m_distinct: "\<And>a. translate node a \<inter> mk_map ps m a = {}"
+      and n_contained: "\<And>a. mk_map ps n a \<subseteq> translate node a"
+  shows "update_one_map ps m n (update_one_map ps n m node) = node"
 proof -
-  have "\<And>a. translate node a - mk_map n a \<subseteq> translate node a" by(auto)
-  hence "\<And>a. (translate node a - mk_map n a) \<inter> mk_map m a 
-                    \<subseteq> translate node a \<inter> mk_map m a"
+  have "\<And>a. translate node a - mk_map ps n a \<subseteq> translate node a" by(auto)
+  hence "\<And>a. (translate node a - mk_map ps n a) \<inter> mk_map ps m a 
+                    \<subseteq> translate node a \<inter> mk_map ps m a"
     by(auto)
   also note m_distinct
-  finally have "\<And>a.(translate node a - mk_map n a) \<inter> mk_map m a = {}" by(auto)
+  finally have "\<And>a.(translate node a - mk_map ps n a) \<inter> mk_map ps m a = {}" by(auto)
   with m_distinct
-  have "\<And>a. translate node a - mk_map n a - mk_map m a =
-             translate node a - mk_map n a"
+  have "\<And>a. translate node a - mk_map ps n a - mk_map ps m a =
+             translate node a - mk_map ps n a"
     by(simp add:Diff_triv)
   with n_contained show ?thesis
     by(simp add:update_one_map_def add_one_map_def remove_one_map_def o_def 
@@ -252,28 +273,28 @@ proof -
 qed    
     
 lemma mk_map_set_append : 
-  "mk_map a aa \<union> \<Union>{mk_map s aa |s. s \<in> set ss} 
-     = \<Union>{mk_map s aa |s. s \<in> set (a # ss)}"
+  "mk_map ps a aa \<union> \<Union>{mk_map ps s aa |s. s \<in> set ss} 
+     = \<Union>{mk_map ps s aa |s. s \<in> set (a # ss)}"
   by(auto)
 
 lemma mk_map_set_commute : 
-  "mk_map a aa \<union> (\<Union>{mk_map s aa |s. s \<in> set ss}\<union> t aa)
-     = \<Union>{mk_map s aa |s. s \<in> set (a # ss)} \<union> t aa"
+  "mk_map ps a aa \<union> (\<Union>{mk_map ps s aa |s. s \<in> set ss}\<union> t aa)
+     = \<Union>{mk_map ps s aa |s. s \<in> set (a # ss)} \<union> t aa"
   by(auto)
     
 lemma translate_update_append: 
-  "translate_update (\<lambda>t aa. \<Union>{mk_map s aa |s. s \<in> set (a # ss)} \<union> t aa) node = 
-  translate_update (\<lambda>t aa. mk_map a aa \<union> (\<Union>{mk_map s aa |s. s \<in> set (ss)}) \<union> t aa) node"
+  "translate_update (\<lambda>t aa. \<Union>{mk_map ps s aa |s. s \<in> set (a # ss)} \<union> t aa) node = 
+  translate_update (\<lambda>t aa. mk_map ps a aa \<union> (\<Union>{mk_map ps s aa |s. s \<in> set (ss)}) \<union> t aa) node"
   by(simp add:mk_map_set_append)
 
 lemma translate_update_commute:  
-  "translate_update (\<lambda>t aa. \<Union>{mk_map s aa |s. s \<in> set (a # ss)} \<union> t aa) node = 
-  translate_update (\<lambda>t aa. mk_map a aa \<union> ((\<Union>{mk_map s aa |s. s \<in> set (ss)}) \<union> t aa)) node"
+  "translate_update (\<lambda>t aa. \<Union>{mk_map ps s aa |s. s \<in> set (a # ss)} \<union> t aa) node = 
+  translate_update (\<lambda>t aa. mk_map ps a aa \<union> ((\<Union>{mk_map ps s aa |s. s \<in> set (ss)}) \<union> t aa)) node"
   by(subst mk_map_set_commute, auto)
     
                                                            
 lemma add_maps_recursive:
-  "add_maps_rec ss node = add_maps ss node"
+  "add_maps_rec ps ss node = add_maps ps ss node"
   apply(induct ss)
   apply(simp_all add:add_maps_def add_maps_rec_def o_def)
   apply(simp add:translate_update_commute[symmetric])
@@ -282,7 +303,7 @@ lemma add_maps_recursive:
 
 (*<*)
 lemma accept_add_maps:
-  "accept (add_maps ms node) = accept node"
+  "accept (add_maps ps ms node) = accept node"
   by(simp add:add_maps_def)
 
     
@@ -292,84 +313,91 @@ lemma translate_update_chain :
   by(simp add:o_def Un_assoc)
 
 lemma add_maps_set_union: 
-     "\<Union>{mk_map s a |s. s \<in> set ms \<or> s \<in> set ns} = 
-      \<Union>{mk_map s a |s. s \<in> set ms} \<union> \<Union>{mk_map s a |s. s \<in> set ns}"      
+     "\<Union>{mk_map ps s a |s. s \<in> set ms \<or> s \<in> set ns} = 
+      \<Union>{mk_map ps s a |s. s \<in> set ms} \<union> \<Union>{mk_map ps s a |s. s \<in> set ns}"      
   by(auto)    
     
 lemma add_maps_set_append :
-      "\<Union>{mk_map s a |s. s \<in> set (ms @ ns)} = 
-       \<Union>{mk_map s a |s. s \<in> set ms} \<union> \<Union>{mk_map s a |s. s \<in> set ns}"    
+      "\<Union>{mk_map ps s a |s. s \<in> set (ms @ ns)} = 
+       \<Union>{mk_map ps s a |s. s \<in> set ms} \<union> \<Union>{mk_map ps s a |s. s \<in> set ns}"    
   by(auto)
   
 lemma add_maps_append_direct:
-   "add_maps ms (add_maps ns node) = 
-    translate_update (\<lambda>t a. \<Union>{mk_map s a |s. s\<in>(set (ms @ ns)) } \<union> t a) node" 
+   "add_maps ps ms (add_maps ps ns node) = 
+    translate_update (\<lambda>t a. \<Union>{mk_map ps s a |s. s\<in>(set (ms @ ns)) } \<union> t a) node" 
   by(simp add:add_maps_def o_def Un_assoc[symmetric] add_maps_set_union)
     
 lemma add_maps_append:
-  "add_maps (ms @ ns) node = add_maps ms (add_maps ns node)"
+  "add_maps ps (ms @ ns) node = add_maps ps ms (add_maps ps ns node)"
   by(simp add:add_maps_def o_def  Un_assoc[symmetric] add_maps_set_union)
 
 lemma add_maps_append2 :
-  "add_maps (a' @ b' @ c' @ d') node = add_maps (a' @ b') (add_maps (c' @ d') node)"
+  "add_maps ps (a' @ b' @ c' @ d') node = add_maps ps (a' @ b') (add_maps  ps(c' @ d') node)"
   by(simp add:add_maps_append)
     
 lemma set_commute: "set [a, b] = set [b, a]"
   by(auto)
     
 lemma add_maps_list_commute :
-  shows   "add_maps [a, b] node = add_maps [b, a] node"
+  shows   "add_maps ps [a, b] node = add_maps ps [b, a] node"
   by(simp only:add_maps_def set_commute)
    
 lemma add_maps_commute:
-  "add_maps (a @ b) node = add_maps (b @ a) node"   
+  "add_maps ps (a @ b) node = add_maps ps (b @ a) node"   
   by(simp only:add_maps_def add_maps_set_append Un_commute)
 
 lemma add_maps_commute3:
-  "add_maps (a @ b @ c) node = add_maps (b @ a @ c) node"   
+  "add_maps ps (a @ b @ c) node = add_maps ps (b @ a @ c) node"   
   apply(simp only:add_maps_def add_maps_set_append)
   apply(simp only:Un_assoc[symmetric])
   apply(simp only: Un_commute)
   done
           
 lemma add_maps_append_commute:
-   "add_maps a (add_maps b node) = add_maps b (add_maps a node)"
+   "add_maps ps a (add_maps ps b node) = add_maps ps b (add_maps ps a node)"
   by(simp add:add_maps_append[symmetric] add_maps_commute)
   
 (*>*)
 
 
-definition mk_node :: "node_spec \<Rightarrow> node"
-  where "mk_node s = add_maps (map_blocks s) 
-                              (add_blocks (acc_blocks s) 
-                              (mk_overlay (overlay s)))"
+definition mk_node :: "property set \<Rightarrow> node_spec \<Rightarrow> node"
+  where "mk_node ps s = add_maps ps (map_blocks s) 
+                         (add_blocks ps (acc_blocks s) 
+                         (mk_overlay (overlay s)))"
+
+text {* the set of used properties in the node is the union of the accept list and 
+        translate list properties*}
+
+definition mk_node_propset :: "node_spec \<Rightarrow> property set"
+  where "mk_node_propset n = mk_map_propset (map_blocks n) \<union> mk_block_propset (acc_blocks n)"
+
 
 (*<*)
 lemma accept_mk_node:
-  "accept (mk_node s) = accept (add_blocks (acc_blocks s) empty_node)"
+  "accept (mk_node ps s) = accept (add_blocks ps (acc_blocks s) empty_node)"
   by(simp add:mk_node_def accept_add_maps add_blocks_overlay)
 
 lemma maps_blocks_comm:
-  "add_maps ms (add_blocks bs node) = add_blocks bs (add_maps ms node)"
+  "add_maps ps ms (add_blocks ps bs node) = add_blocks ps bs (add_maps ps ms node)"
 proof(simp only: add_maps_recursive[symmetric], induct ms, simp_all)
   fix m ms
-  assume IH: "add_maps_rec ms (add_blocks bs node) 
-                  = add_blocks bs (add_maps_rec ms node)"
+  assume IH: "add_maps_rec ps ms (add_blocks ps bs node) 
+                  = add_blocks ps bs (add_maps_rec ps ms node)"
 
   have tu_au_comm:
     "\<And>f g node. translate_update f (accept_update g node) =
                 accept_update g (translate_update f node)"
     by(simp)
 
-  show "translate_update (\<lambda>t a. mk_map m a \<union> t a) 
-                         (add_blocks bs (add_maps_rec ms node)) =
-        add_blocks bs (translate_update (\<lambda>t a. mk_map m a \<union> t a) 
-                                        (add_maps_rec ms node))"
+  show "translate_update (\<lambda>t a. mk_map ps m a \<union> t a) 
+                         (add_blocks ps bs (add_maps_rec ps ms node)) =
+        add_blocks ps bs (translate_update (\<lambda>t a. mk_map ps m a \<union> t a) 
+                                        (add_maps_rec ps ms node))"
     by(induct bs, simp_all add:tu_au_comm)
 qed
 
 lemma translate_mk_node:
-  "translate (mk_node s) = translate (add_maps (map_blocks s) 
+  "translate (mk_node ps s) = translate (add_maps ps (map_blocks s) 
                                      (mk_overlay (overlay s)))"
   by(simp add:mk_node_def maps_blocks_comm translate_add_blocks)
 (*>*)
@@ -382,16 +410,66 @@ primrec repeat_node :: "node_spec \<Rightarrow> nodeid \<Rightarrow> nat \<Right
   where "repeat_node node ba 0 = []" |
         "repeat_node node ba (Suc n) = (ba, node) # repeat_node node (Suc ba) n"
 
+
+text {* we can obtain the relevant properties of the net by the union of all the nodes *}
+
+primrec mk_net_propset :: "net_spec \<Rightarrow> property set"
+  where "mk_net_propset [] = {}" |
+        "mk_net_propset (s#ss) = (mk_net_propset ss) \<union> (mk_node_propset (snd s))"
+
+(*
+primrec mk_net_step :: "property set \<Rightarrow> net_spec \<Rightarrow> net"
+  where "mk_net_step ps [] = empty_net" |
+        "mk_net_step ps (s#ss) = (mk_net_step ps ss)(fst s := mk_node ps (snd s))"
+
+definition mk_net :: "net_spec \<Rightarrow> net"
+  where "mk_net ns = mk_net_step {0..<4} ns"
+*)
+
+definition "relevant_props = {0..<128}"
+
 primrec mk_net :: "net_spec \<Rightarrow> net"
   where "mk_net [] = empty_net" |
-        "mk_net (s#ss) = (mk_net ss)(fst s := mk_node (snd s))"
-
+        "mk_net (s#ss) = (mk_net ss)(fst s := mk_node relevant_props (snd s))"
 
 
 (*<*)
 lemma map_blocks_empty_spec:
   "map_blocks empty_spec = []"
   by(simp add:mk_overlay_def empty_spec_def)
+
+lemma mk_net_empty:
+  "mk_net [] nd = empty_node"
+  by(simp add:mk_net_def empty_net_def)
+
+
+subsubsection {* Finitness of property sets *}
+
+text {* we show that the property sets we obtain from the syntax are finite *}
+
+
+lemma mk_block_propset_finite :
+"finite (mk_block_propset m)"
+  apply(induct m)
+  apply(simp_all add:mk_block_propset_def)
+  done
+
+lemma mk_map_propset_finite:
+"finite (mk_map_propset m)"
+  apply(induct m)
+  apply(simp_all add:mk_map_propset_def)
+  done
+
+lemma mk_node_propset_finite:
+"finite (mk_node_propset n)"
+  by(simp add:mk_node_propset_def mk_map_propset_finite mk_block_propset_finite)
+
+lemma mk_net_propset_finite:
+"finite (mk_net_propset n)"
+  apply(induct n)
+  apply(simp_all add:mk_node_propset_finite mk_net_propset_def)
+  done
+
 
 subsubsection {* Correctness by Construction *}
 
@@ -403,12 +481,11 @@ lemma wf_nodeI:
   "finite (accept node) \<Longrightarrow> (\<And>a. finite (translate node a)) \<Longrightarrow> wf_node node"
   by(simp add:wf_node_def)
 
-
-
 lemma wf_node_wf_net:
   "(\<And>nd. wf_node (net nd)) \<Longrightarrow> wf_net net"
   unfolding wf_node_def wf_net_def 
   by(auto simp:Image_def decodes_to_def decode_step_def)
+
 
 lemma wf_empty_node:
   "wf_node empty_node"
@@ -418,58 +495,60 @@ lemma wf_overlay:
   "wf_node (mk_overlay s)"
   unfolding mk_overlay_def by(cases s, simp_all add:wf_node_def)
 
-
-lemma finite_mk_block:
-"finite (mk_block s)"
-  oops
+lemma mk_block_finite:
+  assumes psfini: "finite ps"
+  shows "finite (mk_block ps s)"
 proof -
-  have sep: "\<And>s. mk_block s = ({a . base s \<le> a 
-                      \<and> a \<le> limit s}) \<times> {p | p . (\<forall>p'\<in> p. p'\<notin> (forbid s))
-                                \<and> (\<forall>p'\<in> (require s). p' \<in> p)}"
-    by(auto simp:mk_block_def)
+  have sep: "{(a, p) | a p. (base s) \<le> a \<and> a \<le> (limit s) 
+               \<and> prop_pred (set (require s)) (set (reject s)) p
+               \<and> p \<subseteq> ps } = {a.(base s) \<le> a \<and> a \<le> (limit s) } \<times>
+                  {p. prop_pred (set (require s)) (set (reject s)) p
+               \<and> p \<subseteq> ps}"
+    by(auto)
+  have fina: "finite {a.(base s) \<le> a \<and> a \<le> (limit s) }"
+    by(auto)
+  from psfini have finb: "finite {p. prop_pred (set (require s)) (set (reject s)) p
+               \<and> p \<subseteq> ps}"
+    by(auto)
 
-
-  have finProps : "finite  {p | p . (\<forall>p'\<in> p. p'\<notin> (forbid s))
-                                \<and> (\<forall>p'\<in> (require s). p' \<in> p)}"
-    by(auto)
-  have finAddrs : "finite ({a . base s \<le> a \<and> a \<le> limit s})"
-    by(auto)
-  from sep finProps finAddrs show ?thesis
-    by(auto)
+  from finb fina sep show ?thesis 
+    by(auto simp: mk_block_def )
 qed
 
 
 lemma wf_add_blocks:
   assumes wf_base: "wf_node node"
-  shows "wf_node (add_blocks ss node)"
+      and psfini: "finite ps"
+  shows "wf_node (add_blocks ps ss node)"
 proof(induct ss, simp_all add:wf_base)
   fix s ss
-  assume IH: "wf_node (add_blocks ss node)"
-  hence "finite (accept (add_blocks ss node))" "\<And>s. finite (translate (add_blocks ss node) s)"
+  assume IH: "wf_node (add_blocks ps ss node)"
+  hence "finite (accept (add_blocks ps ss node))" "\<And>s. finite (translate (add_blocks ps ss node) s)"
     by(auto simp:wf_node_def)
-  moreover have "finite (mk_block s)"
-    by(simp add: finite_mk_block)
-  ultimately show "wf_node (accept_update (op \<union> (mk_block s)) (add_blocks ss node))"
+  moreover from psfini have "finite (mk_block ps s)"
+    by(simp add: mk_block_finite)
+  ultimately show "wf_node (accept_update (op \<union> (mk_block ps s)) (add_blocks ps ss node))"
     by(auto intro:wf_nodeI)
 qed
 
   
 lemma wf_add_maps:
   assumes wf_base: "wf_node node"
-  shows "wf_node (add_maps ss node)"    
+      and psfini: "finite ps"
+  shows "wf_node (add_maps ps ss node)"    
 proof(simp only: add_maps_recursive[symmetric],induct ss, simp_all add:wf_base)
   fix s ss
-  assume IH: "wf_node (add_maps_rec ss node)"
-  hence "finite (accept (add_maps_rec ss node))" "\<And>a. finite (translate (add_maps_rec ss node) a)"
+  assume IH: "wf_node (add_maps_rec ps ss node)"
+  hence "finite (accept (add_maps_rec ps ss node))" "\<And>a. finite (translate (add_maps_rec ps ss node) a)"
     by(auto simp:wf_node_def)
-  moreover have "\<And>a. finite (mk_map s a)"
+  moreover have "\<And>a. finite (mk_map ps s a)"
     unfolding mk_map_def by(simp)
-  ultimately show "wf_node (translate_update (\<lambda>t a. mk_map s a \<union> t a) (add_maps_rec ss node))"
+  ultimately show "wf_node (translate_update (\<lambda>t a. mk_map ps s a \<union> t a) (add_maps_rec ps ss node))"
     by(auto intro:wf_nodeI)
 qed
 
 lemma wf_mk_node:
-  "wf_node (mk_node s)"
+  "finite ps \<Longrightarrow> wf_node (mk_node ps s)"
   unfolding mk_node_def by(auto intro:wf_add_maps wf_add_blocks wf_overlay)
 
 lemma wf_empty_net:
@@ -480,11 +559,29 @@ lemma wf_empty_net:
 
 
 text {* Nets built from abstract syntax are correct by construction: *}
+
+(*
+lemma wf_mk_net_step :
+  assumes psfini: "finite ps"
+  shows "wf_net (mk_net_step ps ss)"
+proof (rule wf_node_wf_net, induct ss)
+  case Nil
+  then show ?case by(auto simp: wf_empty_net empty_net_def wf_empty_node)
+next
+  case (Cons a ss)
+  then show ?case
+    by(simp add:mk_net_step_def wf_mk_node psfini)
+qed
+
 lemma wf_mk_net:
   "wf_net (mk_net ss)"
-(*<*)
-  by(rule wf_node_wf_net, induct ss, simp_all add:empty_net_def wf_empty_node wf_mk_node)
-(*>*)
+  by(simp add:mk_net_def wf_mk_net_step mk_net_propset_finite)
+*)
+
+lemma wf_mk_net:
+  "wf_net (mk_net ss)"
+  by(rule wf_node_wf_net, induct ss, simp_all add:empty_net_def 
+          wf_empty_node wf_mk_node relevant_props_def)
 
 
 
@@ -509,31 +606,31 @@ primrec ff_map :: "map_spec list \<Rightarrow> nodeid"
 (*<*)
 lemma ff_add_blocks_ub:
   assumes "\<And>nd' a' a. (nd',a') \<in> translate node a \<Longrightarrow> nd' < x"
-      and "(nd',a') \<in> translate (add_blocks bs node) a"
+      and "(nd',a') \<in> translate (add_blocks ps bs node) a"
     shows "nd' < x"
   using assms by(simp add:translate_add_blocks)
  
 
 lemma ff_add_maps_ub:
   assumes ff_node: "\<And>nd' a' a. (nd',a') \<in> translate node a \<Longrightarrow> nd' < x"
-      and nda': "(nd',a') \<in> translate (add_maps ms node) a"
+      and nda': "(nd',a') \<in> translate (add_maps ps ms node) a"
     shows "nd' < max x (ff_map ms)"
   using nda'
 proof(induct ms, simp add:ff_node add_maps_recursive[symmetric])
   fix m ms
-  assume IH: "(nd', a') \<in> translate (add_maps ms node) a \<Longrightarrow> nd' < max x (ff_map ms)"
-     and step: "(nd', a') \<in> translate (add_maps (m # ms) node) a"
+  assume IH: "(nd', a') \<in> translate (add_maps ps ms node) a \<Longrightarrow> nd' < max x (ff_map ms)"
+     and step: "(nd', a') \<in> translate (add_maps ps (m # ms) node) a"
      
-  from step have "(nd',a') \<in> mk_map m a \<or> (nd',a') \<in> translate (add_maps ms node) a"
+  from step have "(nd',a') \<in> mk_map ps m a \<or> (nd',a') \<in> translate (add_maps ps ms node) a"
     by(simp add:add_maps_recursive[symmetric])
   thus "nd' < max x (ff_map (m # ms))"
   proof
-    assume "(nd', a') \<in> mk_map m a"
+    assume "(nd', a') \<in> mk_map ps m a"
     hence "nd' < Suc (dest_node m)"
-      by(cases "a \<in> mk_block (src_block m)", simp_all add:mk_map_def)
+      by(cases "a \<in> mk_block ps (src_block m)", simp_all add:mk_map_def)
     thus ?thesis by(simp)
   next
-    assume "(nd', a') \<in> translate (add_maps ms node) a"
+    assume "(nd', a') \<in> translate (add_maps ps ms node) a"
     thus ?thesis by(simp only:add_maps_recursive[symmetric], auto dest:IH)      
   qed
 qed  
@@ -544,7 +641,7 @@ definition ff_node :: "node_spec \<Rightarrow> nodeid"
 
 (*<*)
 lemma ff_node_ub:
-  assumes step: "(nd',a') \<in> translate (mk_node s) a"
+  assumes step: "(nd',a') \<in> translate (mk_node ps s) a"
   shows "nd' < ff_node s"
   unfolding ff_node_def using ff_overlay_ub    
   by(auto simp:translate_add_blocks intro:ff_add_maps_ub[OF _ step[unfolded mk_node_def]])
@@ -557,14 +654,15 @@ primrec ff_net :: "net_spec \<Rightarrow> nodeid"
 (*<*)
 lemma ff_net_empty:
   "ff_net s \<le> nd \<Longrightarrow> mk_net s nd = empty_node"
-  by(induct s, simp_all add:empty_net_def)
+  by(induct s, simp_all add:empty_net_def mk_net_empty)
+
 
 lemma decodes_to_empty_net:
   "decodes_to empty_net = {}"
   by(simp add:decodes_to_def decode_step_def empty_net_def empty_node_def)
 
 lemma ff_net_ub:
-  "(x,y) \<in> decodes_to (mk_net s) \<Longrightarrow> fst x < ff_net s"
+    shows "(x,y) \<in> decodes_to (mk_net s) \<Longrightarrow> fst x < ff_net s"
 proof(induct s, simp add:decodes_to_empty_net)
   fix s ss
   assume IH: "(x, y) \<in> decodes_to (mk_net ss) \<Longrightarrow> fst x < ff_net ss"
@@ -573,18 +671,19 @@ proof(induct s, simp add:decodes_to_empty_net)
   show "fst x < ff_net (s # ss)"
   proof(cases)
     assume "fst y = fst s"
-    with dec have "x \<in> translate (mk_node (snd s)) (snd y)"
-      by(cases x, cases y, simp add:decodes_to_def decode_step_def)
+    with  dec have "x \<in> translate (mk_node relevant_props (snd s)) (snd y)"
+      by(cases x, cases y, simp add:decodes_to_def decode_step_def relevant_props_def)
     hence "fst x < ff_node (snd s)"
       by(cases x, auto intro:ff_node_ub)
     thus ?thesis by(simp)
   next
     assume "fst y \<noteq> fst s"
     with dec have "(x, y) \<in> decodes_to (mk_net ss)"
-      by(cases y, simp add:decodes_to_def decode_step_def)
+      by(cases y, simp add:decodes_to_def decode_step_def mk_net_def)
     with IH show ?thesis by(simp)
   qed
 qed
+
 
 lemma ff_net_fresh:
   assumes ff: "ff_net s \<le> nd"
@@ -598,7 +697,8 @@ proof(intro conjI allI impI)
 next
   fix x y
   assume "(x, y) \<in> decodes_to (mk_net s)"
-  hence "fst x < ff_net s" by(rule ff_net_ub)
+  hence "fst x < ff_net s" 
+    by(rule ff_net_ub)
   also note ff
   finally show "fst x \<noteq> nd" by(simp)
 qed
@@ -619,102 +719,6 @@ proof(induct s, simp_all)
   qed
 qed
 (*>*)
-
-
-subsection "Finiteness of Properties"
-
-primrec block_prop_set :: "block_spec list \<Rightarrow> property set"
-  where "block_prop_set [] = {}" |
-        "block_prop_set (m#mm) = (block_prop_set mm) \<union> set (require m) \<union> set (forbid m)"
-
-lemma block_prop_set_finite :
-"finite (block_prop_set m)"
-  apply(induct m)
-  apply(simp_all add:block_prop_set_def)
-  done
-
-primrec map_prop_set :: "map_spec list \<Rightarrow> property set"
-  where "map_prop_set [] = {}" |
-        "map_prop_set (m#mm) = (map_prop_set mm) \<union> set (propadd m) \<union> set (propstrip m)"
-
-lemma map_prop_set_finite:
-"finite (map_prop_set m)"
-  apply(induct m)
-  apply(simp_all add:map_prop_set_def)
-  done
-
-definition node_prop_set :: "node_spec \<Rightarrow> property set"
-  where "node_prop_set n = map_prop_set (map_blocks n) \<union> block_prop_set (acc_blocks n)"
-
-lemma node_prop_set_finite:
-"finite (node_prop_set n)"
-  by(simp add:node_prop_set_def map_prop_set_finite block_prop_set_finite)
-
-primrec net_prop_set :: "net_spec \<Rightarrow> property set"
-  where "net_prop_set [] = {}" |
-        "net_prop_set (s#ss) = (net_prop_set ss) \<union> (node_prop_set (snd s))"
-
-lemma net_prop_set_finite:
-"finite (net_prop_set n)"
-  apply(induct n)
-  apply(simp_all add:node_prop_set_finite net_prop_set_def)
-  done
-
-lemma "\<exists>N. (net_prop_set n) \<subseteq> {..<N} "
-proof -
-  have fin: "finite (net_prop_set n)"
-    by(simp add: net_prop_set_finite)
-
-  from fin have pred: "\<exists>k. \<forall>p\<in>(net_prop_set n). p < k"
-    by(auto simp: Set_Interval.finite_nat_set_iff_bounded)
-
-  from pred show ?thesis
-    by(auto)  
-qed
-
-
-definition mk_block2 :: "property set \<Rightarrow> block_spec \<Rightarrow> addr set"
-  where "mk_block2 ps s = {(a, p) | a p. (base s) \<le> a \<and> a \<le> (limit s) 
-                                \<and> prop_pred (set (require s)) (set (forbid s)) p
-                                \<and> p \<subseteq> ps }"
-lemma 
-  assumes psfini: "finite ps"
-  shows "finite (mk_block2 ps s)"
-proof -
-  have sep: "{(a, p) | a p. (base s) \<le> a \<and> a \<le> (limit s) 
-               \<and> prop_pred (set (require s)) (set (forbid s)) p
-               \<and> p \<subseteq> ps } = {a.(base s) \<le> a \<and> a \<le> (limit s) } \<times>
-                  {p. prop_pred (set (require s)) (set (forbid s)) p
-               \<and> p \<subseteq> ps}"
-    by(auto)
-  have fina: "finite {a.(base s) \<le> a \<and> a \<le> (limit s) }"
-    by(auto)
-  from psfini have finb: "finite {p. prop_pred (set (require s)) (set (forbid s)) p
-               \<and> p \<subseteq> ps}"
-    by(auto)
-
-  from finb fina sep show ?thesis 
-    by(auto simp: mk_block2_def )
-qed
-    
-
-primrec add_blocks2 :: "property set \<Rightarrow> block_spec list \<Rightarrow> node \<Rightarrow> node"
-  where "add_blocks2 ps [] node = node" |
-        "add_blocks2 ps (s#ss) node = accept_update (op \<union> (mk_block s)) 
-                                                (add_blocks2 ps  ss node)"
-
-definition mk_node2 :: "property set \<Rightarrow> node_spec \<Rightarrow> node"
-  where "mk_node2 ps s = add_maps (map_blocks s) 
-                         (add_blocks2 ps (acc_blocks s) 
-                         (mk_overlay (overlay s)))"
-
-primrec mk_net_step :: "property set \<Rightarrow> net_spec \<Rightarrow> net"
-  where "mk_net_step ps [] = empty_net" |
-        "mk_net_step ps (s#ss) = (mk_net_step ps ss)(fst s := mk_node2 ps (snd s))"
-
-definition mk_net2 :: "net_spec \<Rightarrow> net"
-  where "mk_net2 ns = mk_net_step (net_prop_set ns) ns"
-
 
 
 (*<*)
